

B07-9036 林松角

[1]

$$z = \frac{x - \mu}{\sigma}, f_z(x) = e^{-\frac{1}{2}x^2} \cdot \frac{1}{\sqrt{2\pi}}$$

$$E(z) = 0, E(z - \mu)^2 = 1$$

$$E(z_0 + z_1) = 0, E(z_0 + z_1 - \mu)^2 = 1 + 1 = 2$$

$$(b) Q_1 = z^2 : \chi^2 (df=1)$$

$$(c) Q_2 = z^2 + z_1^2 : \chi^2 (df=2)$$

[2]

$$(a) P(z_0 + z_1 \leq 1) = 0.6914, (1\text{-st, norm.sf}(1, 0, 2))$$

$$(b) P(z_0^2 \leq 1) = 0.8413, (1\text{-st, norm.sf}(1, 0, 1))$$

$$(c) P(z_1^2 + z_2^2 \leq 1) = 0.6914, (1\text{-st, norm.sf}(1, 0, 2))$$

$$(d) P\left(\frac{z_0}{z_1} \leq 1\right)$$

[3]

$$(a) \mu_0 = 65, \frac{s_0^2}{n} = \frac{3^2}{25} = \frac{9}{25}, z = \frac{\bar{x}_0 - 65}{\frac{3}{5}} \quad 4.7\%$$

$$P(\bar{x}_0 \leq 64) = P\left(\frac{\bar{x}_0 - 65}{\frac{3}{5}} \leq \frac{64 - 65}{\frac{3}{5}}\right) = P(z \leq -1.67)$$